okasaki/BootstrappedQueue.ml
@@ -1,13 +1,13 @@
 open Okasaki
 open QueueSig
 
-(*
 
-module BootstrappedQueue : Queue =
+module BootstrappedQueue (* : Queue *) =
 struct
 
    type 'a queues = Empty | Struct of int * 'a list * 'a list Lazy.t queues * int * 'a list 
    type 'a queue = 'a queues
+   type 'a body = int * 'a list * 'a list Lazy.t queues * int * 'a list 
 
    let empty = Empty
 
@@ -15,33 +15,36 @@ struct
      | Empty -> true
      | _ -> false
 
-   let rec checkq ((lenfm, f, m, lenr, r) as q) = 
+   let rec checkq : 'a. 'a body -> 'a queue = 
+      fun ((lenfm, f, m, lenr, r) as q) ->
       if lenr <= lenfm 
          then checkf q
-         else checkf (lenfm+lenr, f, snoc (m, lazy (List.rev r)), 0, [])
+         else checkf (lenfm+lenr, f, snoc m (lazy (List.rev r)), 0, [])
 
-   and checkf (lenfm, f, m, lenr, r) =
+   and checkf : 'a. 'a body -> 'a queue =
+      fun (lenfm, f, m, lenr, r) -> 
       match f, m with
       | [], Empty -> Empty
       | [], _ -> Struct (lenfm, !$(head m), tail m, lenr, r)
       | _ -> Struct (lenfm, f, m, lenr, r)
 
-   and snoc (q:'a queue) (x:'a) = 
+   and snoc : 'a. 'a queue -> 'a -> 'a queue =
+     fun q x ->
       match q with
       | Empty -> Struct (1, [x], Empty, 0, [])
       | Struct (lenfm, f, m, lenr, r) ->
          checkq (lenfm, f, m, lenr+1, x::r)
 
-   and head = function
+   and head : 'a. 'a queue -> 'a = function
       | Empty -> raise EmptyStructure
       | Struct (lenfm, x::f', m, lenr, r) -> x
       | _ -> raise BrokenInvariant
 
-   and tail = function 
+   and tail : 'a. 'a queue -> 'a queue = function 
       | Empty -> raise EmptyStructure
       | Struct (lenfm, x::f', m, lenr, r) -> 
          checkq (lenfm-1, f', m, lenr, r)
       | _ -> raise BrokenInvariant
 
 end
-*)
+
