okasaki/BootstrappedQueue_proof.v
@@ -1,33 +1,47 @@
-Set Bootstrapped Arguments.
+Set Implicit Arguments.
 Require Import FuncTactics LibCore.
 Require Import QueueSig_ml QueueSig_proof.
 Require Import BootstrappedQueue_ml.
 
 (* todo: move, and try to prove implicit queues with it *)
 
-Definition eg_gt_implies (P : (nat->Prop) -> Prop) :=
-  (forall n, (forall m, n > m -> P (eq m)) -> P (gt n).
+Definition eq_gt_implies (P : (nat->Prop) -> Prop) :=
+  forall n, (forall m, n > m -> P (eq m)) -> P (gt n).
 
-Hint Unfold eg_gt_implies.
+Hint Unfold eq_gt_implies.
 
 Lemma eq_gt_induction_2 : forall (P1 P2 : (nat->Prop) -> Prop),
-  eg_gt_implies P1 -> eg_gt_implies P2 ->
+  eq_gt_implies P1 -> eq_gt_implies P2 ->
   (forall n, P1 (gt n) -> P2 (gt n) -> P1 (eq n) /\ P2 (eq n)) ->
   (forall n, P1 (eq n)) /\ (forall n, P2 (eq n)).
-Proof. intros. induction n using peano_induction. auto. Qed. 
+Proof.
+  introv H1 H2 R.
+  cuts M: (forall n, P1 (eq n) /\ P2 (eq n)).
+    split; intros n; specializes M n; auto*.
+  induction n using peano_induction. apply R;
+    match goal with K: eq_gt_implies ?Pi |- ?Pi _ =>
+      apply K; intros; forwards*: H; try math end.
+Qed.
 
 Lemma conj_strengthen_2 : forall (Q1 Q2 P1 P2 : Prop),
   (Q1 -> P1) -> (Q2 -> P2) -> (Q1 /\ Q2) -> (P1 /\ P2).
 Proof. auto*. Qed.
 
 Lemma eq_gt_induction_5 : forall (P1 P2 P3 P4 P5 : (nat->Prop) -> Prop),
-  eg_gt_implies P1 -> eg_gt_implies P2 -> eg_gt_implies P3 -> 
-  eg_gt_implies P4 -> eg_gt_implies P5 ->
+  eq_gt_implies P1 -> eq_gt_implies P2 -> eq_gt_implies P3 -> 
+  eq_gt_implies P4 -> eq_gt_implies P5 ->
   (forall n, P1 (gt n) -> P2 (gt n) -> P3 (gt n) -> P4 (gt n) -> P5 (gt n) -> 
     P1 (eq n) /\ P2 (eq n) /\ P3 (eq n) /\ P4 (eq n) /\ P5 (eq n)) ->
   (forall n, P1 (eq n)) /\ (forall n, P2 (eq n)) /\ (forall n, P3 (eq n))
     /\ (forall n, P4 (eq n))  /\ (forall n, P5 (eq n)).
-Proof. intros. induction n using peano_induction. auto. Qed. 
+Proof. 
+  introv H1 H2 H3 H4 H5 R.
+  cuts M: (forall n, P1 (eq n) /\ P2 (eq n) /\ P3 (eq n) /\ P4 (eq n) /\ P5 (eq n)).
+    splits; intros n; specializes M n; auto*.
+  induction n using peano_induction. apply R;
+    match goal with K: eq_gt_implies ?Pi |- ?Pi _ =>
+      apply K; intros; forwards*: H; try math end.
+Qed. 
 
 Lemma conj_strengthen_5 : forall (Q1 Q2 Q3 Q4 Q5 P1 P2 P3 P4 P5 : Prop),
   (Q1 -> P1) -> (Q2 -> P2) -> (Q3 -> P3) -> (Q4 -> P4) -> (Q5 -> P5) ->
@@ -47,7 +61,7 @@ Import MLBootstrappedQueue.
 Inductive doubling (A:Type) : bool -> int -> list (list A) -> Prop :=
   | doubling_nil : forall first n,
      doubling first n nil
-  | doubling cons : forall first n l ls,
+  | doubling_cons : forall (first:bool) n l ls,
      doubling false (if first then n else 2*n) ls ->
      n <= length l ->
      doubling first n (l::ls).
@@ -55,7 +69,7 @@ Inductive doubling (A:Type) : bool -> int -> list (list A) -> Prop :=
 Inductive inv : bool -> bool -> forall `{Rep a A}, queue a -> list A -> Prop :=
   | inv_empty : forall `{Rep a A} okb okf,
      inv okb okf _ Empty nil
-  | inv_struct : forall `{Rep a A} okb okf lenfm f m lenr r Qf Qr Qms Qm Q,
+  | inv_struct : forall `{Rep a A} (okb okf:bool) lenfm f m lenr r Qf Qr Qms Qm Q,
      Forall2 rep f Qf ->
      Forall2 rep r Qr ->
      inv true true _ m Qms ->
@@ -64,19 +78,19 @@ Inductive inv : bool -> bool -> forall `{Rep a A}, queue a -> list A -> Prop :=
      lenfm =' length Qf + length Qm ->
      Q =' Qf ++ Qm ++ rev Qr ->
      (if okf then f <> nil else True) ->
-     lenr <= lenfm + (if okb then 0 else 1) ->
+     (lenr:int) <= lenfm + (if okb then 0 else 1)->
      doubling true 1 Qms ->
-     inv okb okf _ (Struct lenfm f m lenr r) Q
+     inv okb okf _ (Struct lenfm f m lenr r) Q.
      
 Global Instance queue_rep `{Rep a A} : Rep (queue a) (list A) := 
   inv true true H.
 
 (** automation *)
-Hint Constructors invd inv Forall2.
+Hint Constructors doubling inv Forall2.
 Hint Resolve Forall2_last.
 Hint Extern 1 (@rep (queue _) _ _ _ _) => simpl.
 Hint Extern 1 (@rep (queues _) _ _ _ _) => simpl.
-Ltac auto_tilde ::= eauto.
+Ltac auto_tilde ::= eauto with maths.
 
 (** useful facts *)
 
@@ -88,30 +102,33 @@ Fixpoint depth a (q:queue a) : nat :=
 
 Lemma to_empty : forall `{Rep a A} Q,
   rep Empty Q -> Q = nil.
-Proof. introv RQ. inverts RQ as _ M. inverts~ M. Qed.
+Proof. introv RQ. set_eq Q': Q. inverts~ RQ. Qed.
+  (*todo: bug de inversion ! *)  
 
 Lemma from_empty : forall `{Rep a A} q,
   rep q nil -> q = Empty.
 Proof.
-  introv RQ. inverts RQ as.
-  introv _ ID. inverts~ ID.
-  introv ? ? Df ? ? ?. inverts Df; false.
+  introv RQ. set_eq q': q. inverts RQ as.
+  auto.
+  intros. destruct f. false. inverts H4. false.
 Qed.
 
-Lemma doubling_last_ind : forall A l ls n,
+Lemma doubling_last_ind : forall A (l:list A) ls n,
   doubling false n ls -> 
-  length ls + n <= length l ->
+  length (concat ls) + n <= length l ->
   doubling false n (ls&l).
 Proof.
-  induction ls.
+  induction ls; introv H L; inverts H; rew_list in *; auto~.
 Qed.
 
-Lemma doubling_last : forall A l ls n,
+Lemma doubling_last : forall A (l:list A) ls,
   doubling true 1 ls -> 
-  length ls < length l ->
+  length (concat ls) < length l ->
   doubling true 1 (ls&l).
 Proof.
-  inversion H. apply doubling_last_ind.
+  introv H L. inverts H; rew_list in *.
+  auto~.
+  constructors~. apply~ doubling_last_ind.
 Qed.
 
 (** verification *)
